@@ -1,5 +1,6 @@
 From Stdlib Require Import String List ZArith.
-From imp2lp Require Import Value withvarScalar.SrcLang.
+From imp2lp Require Import Value.
+From imp2lp.withvarScalar Require Import SrcLang Datalog.
 From coqutil Require Import Map.Interface.
 
 Import ListNotations.
@@ -12,25 +13,57 @@ Variant global_rel : Type :=
 
 Variant rel : Type :=
   | glob_rel : global_rel -> rel
-  | aux_rel : nat -> rel.
+  | aux_rel (a : nat).
+(* ???
+Coercion glob_rel : global_rel >-> rel. *)
 
-Coercion glob_rel : global_rel >-> rel.
+Variant fn :=
+  | blit_fn (b : bool)
+  | zlit_fn (z : Z)
+  | nlit_fn (n : nat)
+  | not_fn
+  | and_fn
+  | plus_fn
+  | lt_fn
+  | eq_fn.
 
-Inductive dexpr : Type :=
-| DVar (a : nat)
-| DBool (b : bool)
-| DInt (n : Z)
-| DNot (e : dexpr)
-| DAnd (e1 e2 : dexpr)
-| DPlus (e1 e2 : dexpr)
-| DLt (e1 e2 : dexpr)
-| DEq (e1 e2 : dexpr).
+Definition var := nat.
 
-Record clause :=
-  { clause_rel : rel; clause_args : list dexpr }.
+Variant dvalue : Type :=
+  | DVNat (n : nat)
+  | DVInt (z : Z)
+  | DVBool (b : bool).
 
-Record rule :=
-  { rule_concl : clause; rule_hyps : list clause }.
+Definition dvalue_eqb (a b : dvalue) : bool :=
+  match a, b with
+  | DVInt n1, DVInt n2 => Z.eqb n1 n2
+  | DVBool b1, DVBool b2 => Bool.eqb b1 b2
+  | _, _ => false
+  end.
+
+Definition interp_fun (f : fn) (l : list dvalue) : option dvalue :=
+  match f, l with
+  | blit_fn b, [] => Some (DVBool b)
+  | zlit_fn z, [] => Some (DVInt z)
+  | nlit_fn n, [] => Some (DVNat n)
+  | not_fn, [DVBool b] => Some (DVBool (negb b))
+  | and_fn, [DVBool b1; DVBool b2] => Some (DVBool (andb b1 b2))
+  | plus_fn, [DVInt z1; DVInt z2] => Some (DVInt (z1 + z2))
+  | plus_fn, [DVNat n1; DVNat n2] => Some (DVNat (n1 + n2))
+  | lt_fn, [DVInt z1; DVInt z2] => Some (DVBool (Z.ltb z1 z2))
+  | eq_fn, [v1; v2] => Some (DVBool (dvalue_eqb v1 v2))
+  | _, _ => None
+  end.
+
+Definition aggregator := False.
+Notation dexpr := (Datalog.expr var fn).
+Notation clause := (Datalog.clause rel var fn).
+Notation rule := (Datalog.rule rel var fn aggregator).
+Notation fact := (Datalog.fact rel dvalue).
+
+Instance Sig : signature fn False dvalue :=
+  { interp_fun := interp_fun;
+    interp_agg := fun _ _ => DVNat 0 }.
 
 Definition module := list rule.
 
@@ -46,126 +79,23 @@ Record dprog :=
   { dprog_init : module; dprog_blks : list dblock }.
 (* init to encode initial mut var values and intitial block number *)
 
-Variant dvalue : Type :=
-  | DVBool (b : bool)
-  | DVInt (n : Z).
-
-Definition dvalue_eqb (a b : dvalue) : bool :=
-  match a, b with
-  | DVInt n1, DVInt n2 => Z.eqb n1 n2
-  | DVBool b1, DVBool b2 => Bool.eqb b1 b2
-  | _, _ => false
-  end.
-
-Record fact :=
-  { fact_rel : rel; fact_args : list dvalue }.
-
-Definition mk_fact R args : fact :=
-  {| fact_rel := R; fact_args := args |}.
-
-Unset Elimination Schemes.
-Inductive pftree {T : Type} (P : T -> list T -> Prop) (Q : T -> Prop) : T -> Prop :=
-| pftree_leaf x :
-  Q x ->
-  pftree _ _ x
-| pftree_step x l :
-  P x l ->
-  Forall (pftree _ _) l ->
-  pftree _ _ x.
-Set Elimination Schemes.
-
-Section __.
-  Context (T : Type) (P : T -> list T -> Prop)
-         (Q P0 : T -> Prop).
-  Context (H1: forall x : T, Q x -> P0 x)
-  (H2: forall (x : T) (l : list T),
-      P x l -> Forall (pftree P Q) l -> Forall P0 l -> P0 x).
-
-  Section Tmp.
-    Context(pftree_IS : forall (t: T), pftree P Q t -> P0 t).
-    Fixpoint mk_step_hyp (l : list T) (H : Forall (pftree P Q) l) : Forall P0 l :=
-      match H with
-      | Forall_nil _ => Forall_nil _
-      | Forall_cons _ Hx HFl =>
-          Forall_cons _ (pftree_IS _ Hx) (mk_step_hyp _ HFl)
-      end.
-  End Tmp.
-
-  Fixpoint pftree_IS (t : T)(H : pftree P Q t) : P0 t :=
-    match H with
-    | pftree_leaf _ _ _ HQ => H1 _ HQ
-    | pftree_step _ _ _ l Hl HFl =>
-        H2 _ l Hl HFl (mk_step_hyp pftree_IS l HFl)
-    end.
-End __.
-
-Lemma pftree_ind {U : Type} (P : U -> list U -> Prop) Q R :
-  (forall x, Q x -> R x) ->
-  (forall x l,
-      P x l ->
-      Forall (pftree P Q) l ->
-      Forall R l ->
-      R x) ->
-  forall x, pftree P Q x -> R x.
-Proof.
-  intros H1 H2. fix self 2.
-  intros x Hx. inversion Hx; subst. 1: auto. eapply H2. 1,2: eassumption.
-  clear -H0 self. induction H0; eauto.
-Qed.
-
-Definition union_db {A} (db1 db2 : A -> Prop) :=
-  fun f => db1 f \/ db2 f.
-
-Definition equiv {A} (P Q : A -> Prop) :=
-  forall a, P a <-> Q a.
-
 Section WithMap.
  Context {context : map.map nat dvalue} {context_ok : map.ok context}.
-
- Inductive interp_dexpr (ctx : context) : dexpr -> dvalue -> Prop :=
- | IDVar x v : map.get ctx x = Some v ->
-             interp_dexpr ctx (DVar x) v
- | IDBool b : interp_dexpr ctx (DBool b) (DVBool b)
- | IDInt n : interp_dexpr ctx (DInt n) (DVInt n)
- | IDNot e b : interp_dexpr ctx e (DVBool b) ->
-             interp_dexpr ctx (DNot e) (DVBool (negb b))
- | IDAnd e1 e2 b1 b2 : interp_dexpr ctx e1 (DVBool b1) ->
-                interp_dexpr ctx e2 (DVBool b2) ->
-                interp_dexpr ctx (DAnd e1 e2) (DVBool (andb b1 b2))
- | IDPlus e1 e2 n1 n2 : interp_dexpr ctx e1 (DVInt n1) ->
-                interp_dexpr ctx e2 (DVInt n2) ->
-                interp_dexpr ctx (DPlus e1 e2) (DVInt (n1 + n2))
- | IDLt e1 e2 n1 n2 : interp_dexpr ctx e1 (DVInt n1) ->
-                interp_dexpr ctx e2 (DVInt n2) ->
-                interp_dexpr ctx (DLt e1 e2) (DVBool (Z.ltb n1 n2))
- | IDEq e1 e2 v1 v2 : interp_dexpr ctx e1 v1 ->
-                interp_dexpr ctx e2 v2 ->
-                interp_dexpr ctx (DEq e1 e2) (DVBool (dvalue_eqb v1 v2)).
-
- Variant interp_clause (ctx : context) : clause -> fact -> Prop :=
-   mk_IC c f : c.(clause_rel) = f.(fact_rel) ->
-   Forall2 (interp_dexpr ctx) c.(clause_args) f.(fact_args) ->
-   interp_clause ctx c f.
-
- Definition rule_impl (ctx : context) (rl : rule) (f : fact) (f_hyps : list fact) :=
-   interp_clause ctx rl.(rule_concl) f /\
-     Forall2 (interp_clause ctx) rl.(rule_hyps) f_hyps.
-
- Definition rules_impl (db : fact -> Prop) (rls : list rule) : fact -> Prop :=
-   pftree (fun f f_hyps => exists rl ctx, In rl rls /\ rule_impl ctx rl f f_hyps) db.
 
  Definition mk_asgns_db (db : fact -> Prop) (asgns : list module) (f : fact) : Prop :=
    exists x asgn args,
      nth_error asgns x = Some asgn /\
-       rules_impl db asgn (mk_fact (aux_rel 0) args) /\
-       f = mk_fact (mut_rel x) args.
+       prog_impl asgn db (normal_fact (aux_rel 0) args) /\
+       f = normal_fact (glob_rel (mut_rel x)) args.
 
  Definition mk_flow_db (db : fact -> Prop) (fl : dflow) (f : fact) : Prop :=
    match fl with
-   | DFGoto k => f = mk_fact (blk_rel k) nil
-   | DFIf cond k1 k2 => (rules_impl db cond (mk_fact (aux_rel 0) [DVBool true]) /\ f = mk_fact (blk_rel k1) nil) \/
-                          (rules_impl db cond (mk_fact (aux_rel 0) [DVBool false]) /\ f = mk_fact (blk_rel k2) nil)
-   | DFRet => f = mk_fact terminate_rel nil
+   | DFGoto k => f = normal_fact (glob_rel (blk_rel k)) nil
+   | DFIf cond k1 k2 => (prog_impl cond db (normal_fact (aux_rel 0) [DVBool true]) /\
+                           f = normal_fact (glob_rel (blk_rel k1)) nil) \/
+                          (prog_impl cond db (normal_fact (aux_rel 0) [DVBool false]) /\
+                             f = normal_fact (glob_rel (blk_rel k2)) nil)
+   | DFRet => f = normal_fact (glob_rel terminate_rel) nil
    end.
 
  Fixpoint dblocks_impl (blks : list dblock) (in_db : fact -> Prop) (t : nat) : fact -> Prop :=
@@ -173,23 +103,13 @@ Section WithMap.
    | O => in_db
    | S t => let db := dblocks_impl blks in_db t in
             fun f => exists k blk,
-                db (mk_fact (blk_rel k) nil) /\
+                db (normal_fact (glob_rel (blk_rel k)) nil) /\
                   nth_error blks k = Some blk /\
                   (mk_flow_db db blk.(dblock_fl) f \/
                      mk_asgns_db db blk.(dblock_asgns) f)
    end.
-(* ??? remove
- Inductive dblocks_impl (blks : list dblock) : (fact -> Prop) -> nat -> (fact -> Prop) -> Prop :=
- | DIBase db : dblocks_impl blks db 0 db
- | DIStep db1 db2 db3 t k blk:
-   dblocks_impl blks db1 t db2 ->
-   db2 (mk_fact (blk_rel k) nil) ->
-   nth_error blks k = Some blk ->
-   equiv db3 (union_db (mk_flow_db db2 blk.(dblock_fl)) (mk_asgns_db db2 blk.(dblock_asgns))) ->
-   dblocks_impl blks db1 (S t) db3.
-*)
 
  Definition dprog_impl (prg : dprog) : nat -> fact -> Prop :=
-   let init_db := rules_impl (fun _ => False) prg.(dprog_init) in
+   let init_db := prog_impl prg.(dprog_init) (fun _ => False) in
    dblocks_impl prg.(dprog_blks) init_db.
 End WithMap.
